# Theoretical Derivation of Functional Equation for L_M(s)

**Date**: November 16, 2025
**Status**: Work in progress - theoretical exploration
**Goal**: Derive γ(s) such that γ(s) L_M(s) = γ(1-s) L_M(1-s)

---

## Starting Point

We have the closed form:
```
L_M(s) = ζ(s)[ζ(s) - 1] - C(s)
```

where:
```
C(s) = Σ_{j=2}^∞ H_{j-1}(s)/j^s
H_j(s) = Σ_{k=1}^j k^(-s)
```

---

## Known Tool: Riemann Zeta Functional Equation

```
ξ(s) = π^(-s/2) Γ(s/2) ζ(s)
```

satisfies:
```
ξ(s) = ξ(1-s)
```

Equivalently:
```
ζ(s) = 2^s π^(s-1) sin(πs/2) Γ(1-s) ζ(1-s)
```

or:
```
π^(-s/2) Γ(s/2) ζ(s) = π^(-(1-s)/2) Γ((1-s)/2) ζ(1-s)
```

---

## Strategy

Transform each component of L_M(s) under s → 1-s:

### Part 1: Transform ζ(s)[ζ(s) - 1]

Let's denote R(s) = ζ(s)[ζ(s) - 1] = ζ(s)² - ζ(s)

Under the functional equation, we can write:
```
ζ(s) = F(s) · ζ(1-s)
```

where:
```
F(s) = 2^s π^(s-1) sin(πs/2) Γ(1-s)
```

Then:
```
R(s) = ζ(s)² - ζ(s)
     = F(s)² ζ(1-s)² - F(s) ζ(1-s)
     = F(s) ζ(1-s) [F(s) ζ(1-s) - 1]
```

Similarly:
```
R(1-s) = ζ(1-s)² - ζ(1-s)
```

We want to relate R(s) to R(1-s).

From ζ(s) = F(s) ζ(1-s), we get:
```
ζ(1-s) = ζ(s) / F(s)
```

So:
```
R(1-s) = ζ(1-s)[ζ(1-s) - 1]
       = [ζ(s)/F(s)] · [ζ(s)/F(s) - 1]
       = [ζ(s)/F(s)] · [(ζ(s) - F(s))/F(s)]
       = ζ(s)[ζ(s) - F(s)] / F(s)²
```

Therefore:
```
R(s) / R(1-s) = F(s)² ζ(1-s) [F(s) ζ(1-s) - 1] / {ζ(s)[ζ(s) - F(s)] / F(s)²}
              = F(s)⁴ ζ(1-s) [F(s) ζ(1-s) - 1] / [ζ(s)(ζ(s) - F(s))]
```

This is getting very complex. Let me try a different approach.

---

## Alternative Approach: Use Mellin Transform Properties

The functional equation for Dirichlet series often comes from theta function transformations.

For M(n) = ⌊(τ(n)-1)/2⌋, we might look for a theta function:
```
θ_M(t) = Σ_{n=1}^∞ M(n) e^(-n²πt)
```

Then Mellin transform gives L_M(s), and Poisson summation might give functional equation.

But this requires understanding θ_M(1/t) transformation, which is non-trivial for non-multiplicative M(n).

---

## Direct Approach: Analyze the Correction Sum C(s)

Let's focus on:
```
C(s) = Σ_{j=2}^∞ H_{j-1}(s)/j^s
```

where:
```
H_{j-1}(s) = Σ_{k=1}^{j-1} k^(-s) = ζ(s) - Σ_{k=j}^∞ k^(-s}
```

So:
```
C(s) = Σ_{j=2}^∞ [ζ(s) - Σ_{k=j}^∞ k^(-s}] / j^s
     = ζ(s) Σ_{j=2}^∞ j^(-s) - Σ_{j=2}^∞ j^(-s) Σ_{k=j}^∞ k^(-s}
     = ζ(s) [ζ(s) - 1] - Σ_{j=2}^∞ j^(-s) Σ_{k=j}^∞ k^(-s}
```

So our closed form becomes:
```
L_M(s) = ζ(s)[ζ(s) - 1] - ζ(s)[ζ(s) - 1] + Σ_{j=2}^∞ j^(-s) Σ_{k=j}^∞ k^(-s}
       = Σ_{j=2}^∞ j^(-s) Σ_{k=j}^∞ k^(-s}
```

Wait, that's just a double sum! Let me verify this algebra...

Actually, I made an error. Let me recalculate:

C(s) = Σ_{j=2}^∞ H_{j-1}(s)/j^s

H_{j-1}(s) = Σ_{k=1}^{j-1} k^(-s)

So:
C(s) = Σ_{j=2}^∞ [Σ_{k=1}^{j-1} k^(-s}] / j^s

Let me change the order of summation. For each k, it appears in sums where j > k:

C(s) = Σ_{k=1}^∞ k^(-s) Σ_{j=k+1}^∞ j^(-s}

Now:
Σ_{j=k+1}^∞ j^(-s} = ζ(s) - Σ_{j=1}^k j^(-s} = ζ(s) - H_k(s)

So:
C(s) = Σ_{k=1}^∞ k^(-s) [ζ(s) - H_k(s)]
     = ζ(s) Σ_{k=1}^∞ k^(-s) - Σ_{k=1}^∞ k^(-s) H_k(s)
     = ζ(s)² - Σ_{k=1}^∞ k^(-s) H_k(s)

Therefore:
L_M(s) = ζ(s)[ζ(s) - 1] - C(s)
       = ζ(s)² - ζ(s) - ζ(s)² + Σ_{k=1}^∞ k^(-s) H_k(s)
       = -ζ(s) + Σ_{k=1}^∞ k^(-s) H_k(s)

Hmm, this doesn't match what we expect. Let me check the original closed form derivation...

---

## Next Steps

1. Verify the closed form algebra carefully
2. Try numerical test: Does C(s) = ζ(s)[ζ(s)-1] - Σ_{k=1}^∞ k^(-s} H_k(s)?
3. If algebra checks out, apply FR transformation to the double sum form
4. Look for patterns in how nested zeta sums transform

**Status**: Need to verify algebra before proceeding with FR derivation.
