# Theoretical Derivation of Functional Equation for L_M(s)

**Date**: November 16, 2025, 03:00 CET
**Status**: Work in progress - systematic theoretical approach
**Goal**: Derive γ(s) such that γ(s) L_M(s) = γ(1-s) L_M(1-s)

---

## Verified Starting Point

Closed form (numerically verified):
```
L_M(s) = ζ(s)[ζ(s) - 1] - Σ_{j=2}^∞ H_{j-1}(s)/j^s
```

where H_j(s) = Σ_{k=1}^j k^{-s} is the partial zeta sum.

---

## Known Tool: Riemann Zeta Functional Equation

The Riemann zeta function satisfies:
```
π^{-s/2} Γ(s/2) ζ(s) = π^{-(1-s)/2} Γ((1-s)/2) ζ(1-s)
```

Equivalently:
```
ζ(s) = χ(s) ζ(1-s)
```

where the functional equation factor is:
```
χ(s) = 2^s π^{s-1} sin(πs/2) Γ(1-s)
```

---

## Strategy

We need to find the transformation of the correction sum C(s) under s → 1-s:
```
C(s) = Σ_{j=2}^∞ H_{j-1}(s)/j^s
```

### Step 1: Express C(s) differently

Using H_{j-1}(s) = ζ(s) - TailZeta[s,j] where TailZeta[s,j] = Σ_{k=j}^∞ k^{-s}:

```
C(s) = Σ_{j=2}^∞ [ζ(s) - TailZeta[s,j]]/j^s
     = ζ(s) Σ_{j=2}^∞ j^{-s} - Σ_{j=2}^∞ j^{-s} TailZeta[s,j]
     = ζ(s)[ζ(s) - 1] - Σ_{j=2}^∞ j^{-s} Σ_{k=j}^∞ k^{-s}
```

Therefore:
```
L_M(s) = ζ(s)[ζ(s) - 1] - C(s)
       = ζ(s)[ζ(s) - 1] - [ζ(s)(ζ(s) - 1) - Σ_{j=2}^∞ j^{-s} Σ_{k=j}^∞ k^{-s}]
       = Σ_{j=2}^∞ j^{-s} Σ_{k=j}^∞ k^{-s}
```

**This is a double sum form!**

### Step 2: Double sum analysis

```
L_M(s) = Σ_{j=2}^∞ j^{-s} Σ_{k=j}^∞ k^{-s}
```

Change variables: Let k = j + m where m ≥ 0:
```
L_M(s) = Σ_{j=2}^∞ j^{-s} Σ_{m=0}^∞ (j+m)^{-s}
```

This doesn't immediately simplify with functional equation.

### Step 3: Alternative approach - use partial sums directly

Go back to:
```
C(s) = Σ_{j=2}^∞ H_{j-1}(s)/j^s
```

Under s → 1-s, we need:
```
C(1-s) = Σ_{j=2}^∞ H_{j-1}(1-s)/j^{1-s}
```

Key question: Can we relate H_j(s) to H_j(1-s) using the functional equation?

**Observation**: H_j(s) is a finite sum, so it doesn't have a simple functional equation like ζ(s) does.

However, we know:
```
H_j(s) = Σ_{k=1}^j k^{-s}
```

This is related to the Hurwitz zeta function or polylogarithm, but the finite nature makes it tricky.

---

## Attempt 4: Look for empirical pattern first

Before diving deeper theoretically, let's ask: What would γ(s) need to be?

From the requirement γ(s) L_M(s) = γ(1-s) L_M(1-s), we have:
```
γ(s)/γ(1-s) = L_M(1-s)/L_M(s)
```

The ratio L_M(1-s)/L_M(s) can be computed numerically and might reveal the structure of γ(s).

---

## Next Steps for Theoretical Work

1. **Hurwitz zeta approach**: Express H_j(s) using Hurwitz zeta ζ(s,a) or related functions
2. **Mellin transform**: Use integral representation of L_M(s)
3. **Theta function**: Look for a theta function whose Mellin transform is L_M(s)
4. **Empirical guidance**: Compute L_M(1-s)/L_M(s) for various s to see pattern in γ(s)

---

## Why this is hard

The non-multiplicativity of M(n) means:
- No Euler product
- No simple convolution structure
- The correction sum C(s) doesn't factor nicely
- Partial sums H_j(s) don't have functional equations

However, the Schwarz symmetry we observed suggests FR exists - we just need to find the right approach.

---

**Status**: Theoretical derivation is challenging. The double sum form is promising but doesn't immediately yield γ(s).

**Recommendation**: Combine theoretical work with numerical exploration - compute the ratio L_M(1-s)/L_M(s) empirically to guide the theoretical search for γ(s).
