# Functional Equation Derivation for L_M(s)

**Date**: November 16, 2025, 01:00 CET
**Status**: Work in Progress - Theoretical Derivation

---

## Starting Point

We have the closed form:
```
L_M(s) = ζ(s)[ζ(s) - 1] - Σ_{j=2}^∞ H_{j-1}(s)/j^s
```

where:
- `H_j(s) = Σ_{k=1}^j k^(-s)` are partial zeta sums
- `ζ(s)` is the Riemann zeta function

**Goal**: Derive functional equation relating L_M(s) and L_M(1-s)

---

## Known Functional Equation for ζ(s)

The completed zeta function:
```
ξ(s) = π^(-s/2) Γ(s/2) ζ(s)
```

satisfies the functional equation:
```
ξ(s) = ξ(1-s)
```

Equivalently:
```
π^(-s/2) Γ(s/2) ζ(s) = π^(-(1-s)/2) Γ((1-s)/2) ζ(1-s)
```

This gives us:
```
ζ(s) = π^((2s-1)/2) · [Γ((1-s)/2) / Γ(s/2)] · ζ(1-s)
```

Let's denote:
```
R(s) := π^((2s-1)/2) · Γ((1-s)/2) / Γ(s/2)
```

Then: **ζ(s) = R(s) · ζ(1-s)**

---

## Approach 1: Apply FR to ζ(s)² Term

The dominant term in L_M(s) is `ζ(s)[ζ(s)-1] = ζ(s)² - ζ(s)`.

**Under s → 1-s transformation:**

```
ζ(s)² = [R(s) · ζ(1-s)]²
      = R(s)² · ζ(1-s)²
```

And:
```
ζ(s) = R(s) · ζ(1-s)
```

Therefore:
```
ζ(s)² - ζ(s) = R(s)² · ζ(1-s)² - R(s) · ζ(1-s)
               = R(s) · [R(s) · ζ(1-s)² - ζ(1-s)]
               = R(s) · ζ(1-s) · [R(s) · ζ(1-s) - 1]
```

**Key observation:** This is NOT the same as `R(s) · [ζ(1-s)² - ζ(1-s)]`.

The factor is more complex. Let's call:
```
γ₁(s) = R(s) = π^((2s-1)/2) · Γ((1-s)/2) / Γ(s/2)
```

Then:
```
ζ(s)² - ζ(s) = γ₁(s) · ζ(1-s) · [γ₁(s) · ζ(1-s) - 1]
```

---

## Approach 2: Analyze Correction Sum

The correction sum is:
```
Σ_{j=2}^∞ H_{j-1}(s) / j^s
```

**Question**: Does this sum have a functional equation?

Let's write:
```
H_j(s) = Σ_{k=1}^j k^(-s) = Σ_{k=1}^j 1/k^s
```

**Under reflection s → 1-s:**

Each term `k^(-s)` transforms as:
```
k^(-s) → k^(-(1-s)) = k^(s-1) = k^s / k
```

So:
```
H_j(1-s) = Σ_{k=1}^j k^(s-1)
```

This is NOT simply related to H_j(s) unless we have additional structure.

**Alternative**: Express using Hurwitz zeta:
```
H_j(s) = ζ(s) - ζ(s, j+1)
```

where `ζ(s,a)` is Hurwitz zeta. The Hurwitz zeta has a functional equation, but it's more complex.

---

## Approach 3: Direct Conjecture

Based on numerical evidence (Schwarz symmetry on critical line), we conjecture:

**Conjecture**: There exists a factor γ(s) such that:
```
γ(s) · L_M(s) = γ(1-s) · L_M(1-s)
```

**Candidate forms for γ(s):**

1. **Simple Gamma factor** (like ζ):
   ```
   γ(s) = π^(-s/2) Γ(s/2)
   ```

2. **Double factor** (since L_M ~ ζ²):
   ```
   γ(s) = [π^(-s/2) Γ(s/2)]^2
   ```

3. **Modified factor**:
   ```
   γ(s) = π^(-s/2) Γ(s/2) · [some correction for non-multiplicativity]
   ```

4. **Polynomial correction**:
   ```
   γ(s) = s(1-s) · π^(-s/2) Γ(s/2)
   ```

**Numerical testing** (running separately) will identify which form works.

---

## Approach 4: Mellin Transform Method

L-functions often arise as Mellin transforms. For L_M(s):
```
L_M(s) = Σ M(n)/n^s
```

The Mellin transform perspective:
```
L_M(s) = ∫₀^∞ M̃(x) x^(s-1) dx
```

where `M̃(x)` is a smooth approximation to M(n).

**Functional equation via Poisson summation**:

If we can express M(n) using theta functions or modular forms, Poisson summation gives FR.

**Difficulty**: M(n) is not multiplicative, so standard modular form techniques don't directly apply.

---

## Approach 5: Exploit Closed Form Structure

Return to:
```
L_M(s) = ζ(s)² - ζ(s) - Σ_{j=2}^∞ H_{j-1}(s)/j^s
```

**Rewrite using FR for ζ(s):**

Let `ζ(s) = R(s) ζ(1-s)` where `R(s) = π^((2s-1)/2) Γ((1-s)/2)/Γ(s/2)`.

Then:
```
ζ(s)² = R(s)² ζ(1-s)²
ζ(s) = R(s) ζ(1-s)
```

So:
```
ζ(s)² - ζ(s) = R(s)² ζ(1-s)² - R(s) ζ(1-s)
               = R(s) [R(s) ζ(1-s)² - ζ(1-s)]
               = R(s) {R(s) ζ(1-s)² - ζ(1-s)}
```

Compare with ζ(1-s)² - ζ(1-s):
```
ζ(s)² - ζ(s) = R(s) {R(s) ζ(1-s)² - ζ(1-s)}
             ≠ R(s) [ζ(1-s)² - ζ(1-s)]
```

The mismatch comes from the extra `R(s)` factor on ζ(1-s)².

**Key equation:**
```
ζ(s)² - ζ(s) = R(s) · ζ(1-s) · [R(s) · ζ(1-s) - 1]
```

---

## Conjecture: The Full Functional Equation

**Hypothesis**: The correction sum Σ H_j(s)/j^s compensates for the mismatch.

Let's define:
```
C(s) := Σ_{j=2}^∞ H_{j-1}(s)/j^s
```

Then:
```
L_M(s) = ζ(s)² - ζ(s) - C(s)
```

**Conjecture**:
```
γ(s) · L_M(s) = γ(1-s) · L_M(1-s)
```

where:
```
γ(s) = π^(-s/2) Γ(s/2)  [OR a variant thereof]
```

**To prove**: We need to show that C(s) transforms appropriately under s → 1-s.

---

## Next Steps (Theoretical)

1. **Compute FR for C(s)** using Hurwitz zeta functional equation
2. **Verify algebraically** that the pieces combine correctly
3. **Identify exact form of γ(s)** from the algebra
4. **Cross-check with numerical evidence** from search_gamma_factor.wl

---

## Numerical Evidence (Reference)

From `docs/functional-equation-discovery.md`:
- **Schwarz symmetry** holds: L_M(1/2-it) = Conjugate[L_M(1/2+it)]
- Error < 10^-15 on critical line
- This is **necessary** for FR but not sufficient

**Strong indicator**: FR exists, need to find explicit form.

---

**Status**: Derivation in progress, awaiting numerical γ(s) identification

---

*To be continued with explicit calculation...*
