# Proof Attempt: d[Ï„/2] = 2 from Palindrome Center Properties

**Date**: 2025-11-18, late evening
**Goal**: Derive d[Ï„/2] = 2 using m[Ï„/2] = a[Ï„/2] and palindrome symmetry
**Approach**: Combine empirical invariants with CF recurrence

---

## What We Know

### Universal Empirical Invariants (100% tested)

1. **m[Ï„/2] = a[Ï„/2]** at exact center of even period
2. **p - m[Ï„/2]Â² = 2Â·d[Ï„/2-1]** (key identity)
3. **d[Ï„/2] = 2** (what we want to prove)
4. **m[Ï„/2] â‰ˆ âˆšp** (always slightly below)

### Proven Properties

5. **Palindrome**: a_k = a_{Ï„-k}, d_k = d_{Ï„-k}
6. **Recurrence**: a_k = âŒŠ(aâ‚€ + m_k) / d_kâŒ‹
7. **Even period**: Ï„ â‰¡ 0 or 2 (mod 4) for p â‰¡ 3 (mod 4)

---

## Derivation from m = a Invariant

### Step 1: Use the Invariant

At k = Ï„/2, let m = a (by invariant 1).

From recurrence (property 6):
```
a = âŒŠ(aâ‚€ + m) / dâŒ‹
  = âŒŠ(aâ‚€ + a) / dâŒ‹    (substituting m = a)
```

This means:
```
a â‰¤ (aâ‚€ + a) / d < a + 1
```

Multiply by d:
```
aÂ·d â‰¤ aâ‚€ + a < (a+1)Â·d
```

Simplify:
```
aÂ·d - a â‰¤ aâ‚€ < aÂ·d + d - a
aÂ·(d-1) â‰¤ aâ‚€ < aÂ·(d-1) + d
```

**Key inequality**:
```
aÂ·(d-1) â‰¤ aâ‚€ < aÂ·(d-1) + d
```

Since aâ‚€ = âŒŠâˆšpâŒ‹, this constrains d in terms of a.

### Step 2: Solve for d

From the left inequality:
```
aÂ·(d-1) â‰¤ aâ‚€
d - 1 â‰¤ aâ‚€/a
d â‰¤ aâ‚€/a + 1
```

From the right inequality:
```
aâ‚€ < aÂ·(d-1) + d
aâ‚€ < aÂ·d - a + d
aâ‚€ < dÂ·(a+1) - a
d > (aâ‚€ + a) / (a+1)
```

**Combining**:
```
(aâ‚€ + a) / (a+1) < d â‰¤ aâ‚€/a + 1
```

### Step 3: Use m â‰ˆ âˆšp

We know empirically: a = m â‰ˆ âˆšp â‰ˆ aâ‚€

**Approximation**: Let a = aâ‚€ - Îµ for small Îµ â‰¥ 0.

Then:
```
Lower bound: d > (aâ‚€ + aâ‚€ - Îµ) / (aâ‚€ - Îµ + 1)
                = (2aâ‚€ - Îµ) / (aâ‚€ - Îµ + 1)
                â‰ˆ 2aâ‚€ / aâ‚€ = 2  (if Îµ small)

Upper bound: d â‰¤ aâ‚€ / (aâ‚€ - Îµ) + 1
                â‰ˆ 1 + 1 = 2  (if Îµ â‰ˆ 0)
```

**Conclusion**: d â‰ˆ 2 when a â‰ˆ aâ‚€!

### Step 4: Exact Derivation for a = aâ‚€

**Special case**: If a = m = aâ‚€ exactly:
```
Lower bound: d > (aâ‚€ + aâ‚€) / (aâ‚€ + 1) = 2aâ‚€ / (aâ‚€ + 1)
Upper bound: d â‰¤ aâ‚€/aâ‚€ + 1 = 2
```

For large aâ‚€ (large p): 2aâ‚€/(aâ‚€+1) â†’ 2

**Since d must be an integer** and 2aâ‚€/(aâ‚€+1) < d â‰¤ 2:

For aâ‚€ â‰¥ 2: 2aâ‚€/(aâ‚€+1) > 1.33...

**Therefore**: The only integer satisfying this is d = 2! âœ“

---

## Verification with Empirical Data

### Case: a = aâ‚€ - 1

**Common case**: m[Ï„/2] = aâ‚€ - 1

Lower bound:
```
d > (aâ‚€ + aâ‚€ - 1) / (aâ‚€ - 1 + 1)
  = (2aâ‚€ - 1) / aâ‚€
  = 2 - 1/aâ‚€
```

Upper bound:
```
d â‰¤ aâ‚€/(aâ‚€ - 1) + 1
  = aâ‚€/(aâ‚€ - 1) + 1
  â‰ˆ 1 + 1 = 2  (for large aâ‚€)
```

More precisely:
```
For aâ‚€ = 3: d â‰¤ 3/2 + 1 = 2.5 â†’ d = 2
For aâ‚€ = 4: d â‰¤ 4/3 + 1 = 2.33 â†’ d = 2
For aâ‚€ â‰¥ 3: 2 - 1/aâ‚€ < d â‰¤ aâ‚€/(aâ‚€-1) + 1
```

Since aâ‚€/(aâ‚€-1) + 1 < 3 for aâ‚€ â‰¥ 2, and d > 2 - 1/aâ‚€ â‰ˆ 2:

**The only integer is d = 2!** âœ“

### Case: a = aâ‚€ + 1

**Rare case**: m[Ï„/2] = aâ‚€ + 1

Lower bound:
```
d > (aâ‚€ + aâ‚€ + 1) / (aâ‚€ + 2)
  = (2aâ‚€ + 1) / (aâ‚€ + 2)
  â‰ˆ 2  (for large aâ‚€)
```

Upper bound:
```
d â‰¤ aâ‚€/(aâ‚€ + 1) + 1
  < 1 + 1 = 2
```

**Problem**: Lower bound â‰ˆ 2, upper bound < 2!

This case is IMPOSSIBLE if the invariant m = a holds.

**Conclusion**: We never have a > aâ‚€ (consistent with m â‰¤ âˆšp < aâ‚€ + 1).

---

## General Proof (for aâ‚€ - 1 â‰¤ a â‰¤ aâ‚€)

**Claim**: If m = a at position Ï„/2, and aâ‚€ - 1 â‰¤ a â‰¤ aâ‚€, then d = 2.

**Proof**:

From the constraint:
```
aÂ·(d-1) â‰¤ aâ‚€ < aÂ·(d-1) + d
```

**Case 1**: a = aâ‚€
```
aâ‚€Â·(d-1) â‰¤ aâ‚€ < aâ‚€Â·(d-1) + d
d - 1 â‰¤ 1 < d - 1 + d/aâ‚€
d â‰¤ 2 < d + d/aâ‚€ - 1
```
From d â‰¤ 2 and d - 1 < 1 + d/aâ‚€, we get d = 2 (only integer solution).

**Case 2**: a = aâ‚€ - 1
```
(aâ‚€-1)Â·(d-1) â‰¤ aâ‚€ < (aâ‚€-1)Â·(d-1) + d
```
Expand:
```
aâ‚€Â·d - aâ‚€ - d + 1 â‰¤ aâ‚€ < aâ‚€Â·d - aâ‚€ - d + 1 + d
aâ‚€Â·d - 2aâ‚€ - d + 1 â‰¤ 0 < aâ‚€Â·d - 2aâ‚€ + 1
```
From left: aâ‚€Â·d â‰¤ 2aâ‚€ + d - 1
           dÂ·(aâ‚€ - 1) â‰¤ 2aâ‚€ - 1
           d â‰¤ (2aâ‚€ - 1) / (aâ‚€ - 1)

For aâ‚€ â‰¥ 3:
```
(2aâ‚€ - 1) / (aâ‚€ - 1) = (2(aâ‚€ - 1) + 1) / (aâ‚€ - 1)
                      = 2 + 1/(aâ‚€ - 1)
                      â‰¤ 2.5  (for aâ‚€ = 3)
```

From right: aâ‚€Â·d > 2aâ‚€ - 1
            d > 2 - 1/aâ‚€
            d â‰¥ 2  (since d integer and aâ‚€ â‰¥ 2)

**Combining**: 2 â‰¤ d â‰¤ 2 + 1/(aâ‚€-1) < 3

**Therefore**: d = 2! âœ“

---

## Conclusion

**Theorem** (Conditional):

If the following hold at k = Ï„/2:
1. m[Ï„/2] = a[Ï„/2] (empirical invariant)
2. aâ‚€ - 1 â‰¤ a[Ï„/2] â‰¤ aâ‚€ (empirical bound)
3. aâ‚€ â‰¥ 2 (true for all primes p â‰¥ 7)

Then: **d[Ï„/2] = 2**

**Proof**: Direct from the recurrence constraint aÂ·(d-1) â‰¤ aâ‚€ < aÂ·(d-1) + d, as shown above.

---

## Status

**What we've proven**:
âœ… IF m = a at center AND a â‰ˆ aâ‚€, THEN d = 2 (algebraic, rigorous)

**What remains**:
â“ Why does m = a hold at the palindrome center?
â“ Is this a consequence of palindrome symmetry?
â“ Classical CF theorem we're missing?

**Confidence**:
- Conditional proof: 100% rigorous
- Empirical invariants: 100% (25+ tested)
- Overall: Very high confidence, likely classical result

---

## Implications

**For main theorem** (xâ‚€ â‰¡ +1 mod p for p â‰¡ 7 mod 8):

1. âœ… PROVEN: Period Ï„ â‰¡ 0 (mod 4) [Legendre symbols]
2. ðŸ”¬ EMPIRICAL: m = a at Ï„/2 [25+ cases]
3. âœ… PROVEN: If m = a and a â‰ˆ aâ‚€, then d = 2 [this document]
4. âœ… PROVEN: d = 2 implies norm = +2 [Euler's formula]
5. âœ… PROVEN: Norm = +2 implies xâ‚€ â‰¡ +1 [half-period formula]

**Missing link**: Prove m = a from first principles (palindrome theory).

**Alternatively**: Accept m = a as empirical, then entire chain is proven modulo this single invariant.

---

**Next**: Either find classical reference for m = a at palindrome center, or investigate palindrome symmetry argument more deeply.
